ver2/memory_ops_solvers_impl.v
@@ -40,110 +40,95 @@ Import SymbolicStateCmp.
 Module MemoryOpsSolversImpl.
 
 (* Doesn't check the memory for the value, just returns an abstract load *)
-Definition basic_mload_solver: mload_solver_type :=
-  fun (soffset: sstack_val) =>
-  fun (smem: smemory) =>
-  fun (instk_height: nat) =>
-  fun (m: smap) =>
-  fun (ops: stack_op_instr_map) =>
-  SymMLOAD soffset smem.
-
-Lemma basic_mload_solver_snd: mload_solver_snd basic_mload_solver.
-Admitted.
+  Definition trivial_mload_solver (sstack_val_cmp: sstack_val_cmp_ext_1_t) (soffset: sstack_val) (smem: smemory) (instk_height: nat) (m: smap) (ops: stack_op_instr_map) :=
+    SymMLOAD soffset smem.
 
 (* Doesn't check the memory, just appends the abstract store *)
-Definition basic_smemory_updater: smemory_updater_type :=
-  fun (update: memory_update sstack_val) =>
-  fun (smem: smemory) =>
-  fun (instk_height: nat) =>
-  fun (m: smap) =>
-  fun (ops: stack_op_instr_map) =>
-  (update::smem).
-
-Lemma basic_smemory_updater_snd: smemory_updater_snd basic_smemory_updater.
-Admitted.
+  Definition trivial_smemory_updater (sstack_val_cmp: sstack_val_cmp_ext_1_t) (update: memory_update sstack_val) (smem: smemory) (instk_height: nat) (m: smap) (ops: stack_op_instr_map) :=
+      (update::smem).
 
 
-Definition mstore_updates_do_not_overlap (soffset soffset': sstack_val) : bool :=
-  match soffset, soffset' with
-  | Val v1, Val v2 =>
-      let addr := (wordToN v1) in
-      let addr' := (wordToN v2) in
-      orb (addr+31 <? addr')%N (addr'+31 <? addr)%N
-  | _, _ => false
-  end.
 
-Definition mstore8_updates_do_not_overlap (soffset soffset': sstack_val) : bool :=
-  match soffset, soffset' with
-  | Val v1, Val v2 =>
-      let addr := (wordToN v1) in
-      let addr' := (wordToN v2) in
-      orb (addr <? addr')%N (addr'+31 <? addr)%N
-  | _, _ => false
-  end.
-
-Definition mstore8_is_included_in_mstore (soffset_mstore8 soffset_mstore: sstack_val) : bool :=
-  match soffset_mstore8, soffset_mstore with
-  | Val v1, Val v2 =>
-      let addr_mstore8 := (wordToN v1) in
-      let addr_mstore := (wordToN v2) in
-      andb (addr_mstore <=? addr_mstore8 )%N (addr_mstore8 <=? addr_mstore+31)%N
-  | _, _ => false
-  end.
-
-Fixpoint adv_mload_solver (sstack_val_cmp: sstack_val_cmp_ext_1_t) (soffset: sstack_val) (smem: smemory) (instk_height: nat) (m: smap) (ops: stack_op_instr_map) :=
-  match smem with
-  | [] => SymMLOAD soffset []
-  | (U_MSTORE _ soffset' svalue)::smem' =>
-      if sstack_val_cmp (S (get_maxidx_smap m)) soffset soffset' (get_maxidx_smap m) (get_bindings_smap m) (get_maxidx_smap m) (get_bindings_smap m) instk_height ops then
-        SymBasicVal svalue
-      else
-        if mstore_updates_do_not_overlap soffset soffset' then
-          adv_mload_solver sstack_val_cmp soffset smem' instk_height m ops
+  Definition mstore_updates_do_not_overlap (soffset soffset': sstack_val) : bool :=
+    match soffset, soffset' with
+    | Val v1, Val v2 =>
+        let addr := (wordToN v1) in
+        let addr' := (wordToN v2) in
+        orb (addr+31 <? addr')%N (addr'+31 <? addr)%N
+    | _, _ => false
+    end.
+  
+  Definition mstore8_updates_do_not_overlap (soffset soffset': sstack_val) : bool :=
+    match soffset, soffset' with
+    | Val v1, Val v2 =>
+        let addr := (wordToN v1) in
+        let addr' := (wordToN v2) in
+        orb (addr <? addr')%N (addr'+31 <? addr)%N
+    | _, _ => false
+    end.
+  
+  Definition mstore8_is_included_in_mstore (soffset_mstore8 soffset_mstore: sstack_val) : bool :=
+    match soffset_mstore8, soffset_mstore with
+    | Val v1, Val v2 =>
+        let addr_mstore8 := (wordToN v1) in
+        let addr_mstore := (wordToN v2) in
+        andb (addr_mstore <=? addr_mstore8 )%N (addr_mstore8 <=? addr_mstore+31)%N
+    | _, _ => false
+    end.
+  
+  Fixpoint basic_mload_solver (sstack_val_cmp: sstack_val_cmp_ext_1_t) (soffset: sstack_val) (smem: smemory) (instk_height: nat) (m: smap) (ops: stack_op_instr_map) :=
+    match smem with
+    | [] => SymMLOAD soffset []
+    | (U_MSTORE _ soffset' svalue)::smem' =>
+        if sstack_val_cmp (S (get_maxidx_smap m)) soffset soffset' (get_maxidx_smap m) (get_bindings_smap m) (get_maxidx_smap m) (get_bindings_smap m) instk_height ops then
+          SymBasicVal svalue
         else
-          SymMLOAD soffset' smem
-  | (U_MSTORE8 _ soffset' svalue)::smem' =>
-      if mstore8_updates_do_not_overlap soffset soffset' then
-        adv_mload_solver sstack_val_cmp soffset smem' instk_height m ops
-      else
-        SymMLOAD soffset' smem             
-  end.
-
-
-Fixpoint adv_smemory_updater_remove_mstore_dups (sstack_val_cmp: sstack_val_cmp_ext_1_t) (soffset_mstore: sstack_val) (smem: smemory) (instk_height: nat) (m: smap) (ops: stack_op_instr_map) :=
-  match smem with
-  | [] => []
-  | (U_MSTORE _ soffset' svalue)::smem' =>
-      if sstack_val_cmp (S (get_maxidx_smap m)) soffset_mstore soffset' (get_maxidx_smap m) (get_bindings_smap m) (get_maxidx_smap m) (get_bindings_smap m) instk_height ops then
-        adv_smemory_updater_remove_mstore_dups sstack_val_cmp soffset_mstore smem' instk_height m ops (* we can also stop, since we will have at most one duplicate *)
-      else
-        (U_MSTORE sstack_val soffset' svalue)::(adv_smemory_updater_remove_mstore_dups sstack_val_cmp soffset_mstore smem' instk_height m ops)
-  | (U_MSTORE8 _ soffset' svalue)::smem' =>
-      if mstore8_is_included_in_mstore soffset' soffset_mstore then
-        adv_smemory_updater_remove_mstore_dups sstack_val_cmp soffset_mstore smem' instk_height m ops (* we can also stop, since we will have at most one duplicate *)
-      else
-        (U_MSTORE8 sstack_val soffset' svalue)::(adv_smemory_updater_remove_mstore_dups sstack_val_cmp soffset_mstore smem' instk_height m ops)
-  end.
-
-Fixpoint adv_smemory_updater_remove_mstore8_dups (sstack_val_cmp: sstack_val_cmp_ext_1_t) (soffset_mstore8: sstack_val) (smem: smemory) (instk_height: nat) (m: smap) (ops: stack_op_instr_map) :=
-  match smem with
-  | [] => []
-  | (U_MSTORE8 _ soffset' svalue)::smem' =>
-      if sstack_val_cmp (S (get_maxidx_smap m)) soffset_mstore8 soffset' (get_maxidx_smap m) (get_bindings_smap m) (get_maxidx_smap m) (get_bindings_smap m) instk_height ops then
-        adv_smemory_updater_remove_mstore8_dups sstack_val_cmp soffset_mstore8 smem' instk_height m ops (* we can also stop, since we will have at most one duplicate *)
-      else
-        (U_MSTORE8 sstack_val soffset' svalue)::(adv_smemory_updater_remove_mstore8_dups sstack_val_cmp soffset_mstore8 smem' instk_height m ops)
-  | (U_MSTORE _ soffset' svalue)::smem' =>
-        (U_MSTORE sstack_val soffset' svalue)::(adv_smemory_updater_remove_mstore8_dups sstack_val_cmp soffset_mstore8 smem' instk_height m ops)
-  end.
-
-Definition adv_smemory_updater (sstack_val_cmp: sstack_val_cmp_ext_1_t) (update: memory_update sstack_val) (smem: smemory) (instk_height: nat) (m: smap) (ops: stack_op_instr_map) :=
-  match update with
-  | U_MSTORE _ soffset _ =>
-      update::(adv_smemory_updater_remove_mstore_dups sstack_val_cmp soffset smem instk_height m ops)
-  | U_MSTORE8 _ soffset _ =>
-      update::(adv_smemory_updater_remove_mstore8_dups sstack_val_cmp soffset smem instk_height m ops)
-  end.
-
+          if mstore_updates_do_not_overlap soffset soffset' then
+            basic_mload_solver sstack_val_cmp soffset smem' instk_height m ops
+          else
+            SymMLOAD soffset' smem
+    | (U_MSTORE8 _ soffset' svalue)::smem' =>
+        if mstore8_updates_do_not_overlap soffset soffset' then
+          basic_mload_solver sstack_val_cmp soffset smem' instk_height m ops
+        else
+          SymMLOAD soffset' smem             
+    end.
+  
+  
+  Fixpoint basic_smemory_updater_remove_mstore_dups (sstack_val_cmp: sstack_val_cmp_ext_1_t) (soffset_mstore: sstack_val) (smem: smemory) (instk_height: nat) (m: smap) (ops: stack_op_instr_map) :=
+    match smem with
+    | [] => []
+    | (U_MSTORE _ soffset' svalue)::smem' =>
+        if sstack_val_cmp (S (get_maxidx_smap m)) soffset_mstore soffset' (get_maxidx_smap m) (get_bindings_smap m) (get_maxidx_smap m) (get_bindings_smap m) instk_height ops then
+          basic_smemory_updater_remove_mstore_dups sstack_val_cmp soffset_mstore smem' instk_height m ops (* we can also stop, since we will have at most one duplicate *)
+        else
+          (U_MSTORE sstack_val soffset' svalue)::(basic_smemory_updater_remove_mstore_dups sstack_val_cmp soffset_mstore smem' instk_height m ops)
+    | (U_MSTORE8 _ soffset' svalue)::smem' =>
+        if mstore8_is_included_in_mstore soffset' soffset_mstore then
+          basic_smemory_updater_remove_mstore_dups sstack_val_cmp soffset_mstore smem' instk_height m ops (* we can also stop, since we will have at most one duplicate *)
+        else
+          (U_MSTORE8 sstack_val soffset' svalue)::(basic_smemory_updater_remove_mstore_dups sstack_val_cmp soffset_mstore smem' instk_height m ops)
+    end.
+  
+  Fixpoint basic_smemory_updater_remove_mstore8_dups (sstack_val_cmp: sstack_val_cmp_ext_1_t) (soffset_mstore8: sstack_val) (smem: smemory) (instk_height: nat) (m: smap) (ops: stack_op_instr_map) :=
+    match smem with
+    | [] => []
+    | (U_MSTORE8 _ soffset' svalue)::smem' =>
+        if sstack_val_cmp (S (get_maxidx_smap m)) soffset_mstore8 soffset' (get_maxidx_smap m) (get_bindings_smap m) (get_maxidx_smap m) (get_bindings_smap m) instk_height ops then
+          basic_smemory_updater_remove_mstore8_dups sstack_val_cmp soffset_mstore8 smem' instk_height m ops (* we can also stop, since we will have at most one duplicate *)
+        else
+          (U_MSTORE8 sstack_val soffset' svalue)::(basic_smemory_updater_remove_mstore8_dups sstack_val_cmp soffset_mstore8 smem' instk_height m ops)
+    | (U_MSTORE _ soffset' svalue)::smem' =>
+        (U_MSTORE sstack_val soffset' svalue)::(basic_smemory_updater_remove_mstore8_dups sstack_val_cmp soffset_mstore8 smem' instk_height m ops)
+    end.
+  
+  Definition basic_smemory_updater (sstack_val_cmp: sstack_val_cmp_ext_1_t) (update: memory_update sstack_val) (smem: smemory) (instk_height: nat) (m: smap) (ops: stack_op_instr_map) :=
+    match update with
+    | U_MSTORE _ soffset _ =>
+        update::(basic_smemory_updater_remove_mstore_dups sstack_val_cmp soffset smem instk_height m ops)
+    | U_MSTORE8 _ soffset _ =>
+        update::(basic_smemory_updater_remove_mstore8_dups sstack_val_cmp soffset smem instk_height m ops)
+    end.
+  
 
 End MemoryOpsSolversImpl.
