ver2/block_equiv_checker.v
@@ -1,0 +1,246 @@
+Require Import FORVES.program.
+Import Program.
+
+Require Import FORVES.stack_operation_instructions.
+Import StackOpInstrs.
+
+Require Import FORVES.execution_state.
+Import ExecutionState.
+
+Require Import FORVES.concrete_interpreter.
+Import ConcreteInterpreter.
+
+Require Import FORVES.optimizations_def.
+Import Optimizations_Def.
+
+Require Import FORVES.symbolic_execution.
+Import SymbolicExecution.
+
+Require Import FORVES.storage_ops_solvers.
+Import StorageOpsSolvers.
+
+Require Import FORVES.storage_ops_solvers_impl.
+Import StorageOpsSolversImpl.
+
+Require Import FORVES.memory_ops_solvers.
+Import MemoryOpsSolvers.
+
+Require Import FORVES.memory_ops_solvers_impl.
+Import MemoryOpsSolversImpl.
+
+Require Import FORVES.symbolic_state_cmp.
+Import SymbolicStateCmp.
+
+Require Import FORVES.valid_symbolic_state.
+Import ValidSymbolicState.
+
+Require Import FORVES.symbolic_execution_soundness.
+Import SymbolicExecutionSoundness.
+
+Require Import FORVES.symbolic_state_eval.
+Import SymbolicStateEval.
+
+Require Import FORVES.symbolic_state.
+Import SymbolicState.
+
+Require Import FORVES.symbolic_state_cmp_impl.
+Import SymbolicStateCmpImpl.
+
+Require Import FORVES.sstack_val_cmp_impl.
+Import SStackValCmpImpl.
+
+Require Import FORVES.sstack_val_cmp_impl_soundness.
+Import SStackValCmpImplSoundness.
+
+Require Import FORVES.sha3_cmp_impl.
+Import SHA3CmpImpl.
+
+Require Import FORVES.sha3_cmp_impl_soundness.
+Import SHA3CmpImplSoundness.
+
+Require Import FORVES.storage_cmp_impl.
+Import StorageCmpImpl.
+
+Require Import FORVES.storage_cmp_impl_soundness.
+Import StorageCmpImplSoundness.
+
+
+Require Import FORVES.memory_cmp_impl.
+Import MemoryCmpImpl.
+
+Require Import FORVES.memory_cmp_impl_soundness.
+Import MemoryCmpImplSoundness.
+
+Require Import FORVES.storage_ops_solvers_impl.
+Import StorageOpsSolversImpl.
+
+Require Import FORVES.storage_ops_solvers_impl_soundness.
+Import StorageOpsSolversImplSoundness.
+
+Require Import FORVES.memory_ops_solvers_impl.
+Import MemoryOpsSolversImpl.
+
+Require Import FORVES.memory_ops_solvers_impl_soundness.
+Import MemoryOpsSolversImplSoundness.
+
+
+
+Require Import FORVES.misc.
+Import Misc.
+
+Module BlockEquivChecker.
+
+
+  (* mload solvers *)
+  Inductive mload_solver_v :=
+  | MLoadSolver (f: mload_solver_ext_type) (H_snd: mload_solver_ext_snd f).
+
+  Inductive available_mload_solvers :=
+  | MLoadSolver_Trivial
+  | MLoadSolver_Basic.
+
+  Definition get_mload_solver (tag: available_mload_solvers) : mload_solver_v :=
+    match tag with
+    | MLoadSolver_Trivial => MLoadSolver trivial_mload_solver trivial_mload_solver_snd
+    | MLoadSolverStrgUpdater_Basic => MLoadSolver basic_mload_solver basic_mload_solver_snd
+  end.
+
+  (* sload solvers *)
+  Inductive sload_solver_v :=
+  | SLoadSolver (f: sload_solver_ext_type) (H_snd: sload_solver_ext_snd f).
+
+  Inductive available_sload_solvers :=
+  | SLoadSolver_Trivial
+  | SLoadSolver_Basic.
+
+  Definition get_sload_solver (tag: available_sload_solvers) : sload_solver_v :=
+    match tag with
+    | SLoadSolver_Trivial => SLoadSolver trivial_sload_solver trivial_sload_solver_snd
+    | SLoadSolverStrgUpdater_Basic => SLoadSolver basic_sload_solver basic_sload_solver_snd
+  end.
+
+  (* memory updaters *)
+  Inductive smemory_updater_v :=
+  | SMemUpdater (f: smemory_updater_ext_type) (H_snd: smemory_updater_ext_snd f).
+
+  Inductive available_smemory_updaters :=
+  | SMemUpdater_Trivial
+  | SMemUpdater_Basic.
+
+  Definition get_smemory_updater (tag: available_smemory_updaters) : smemory_updater_v :=
+    match tag with
+    | SMemUpdater_Trivial => SMemUpdater trivial_smemory_updater trivial_smemory_updater_snd
+    | SMemUpdater_Basic => SMemUpdater basic_smemory_updater basic_smemory_updater_snd
+  end.
+
+  (* storage updaters *)
+  Inductive sstorage_updater_v :=
+  | SStrgUpdater (f: sstorage_updater_ext_type) (H_snd: sstorage_updater_ext_snd f).
+
+  Inductive available_sstorage_updaters :=
+  | SStrgUpdater_Trivial
+  | SStrgUpdater_Basic.
+
+  Definition get_sstorage_updater (tag: available_sstorage_updaters) : sstorage_updater_v :=
+    match tag with
+    | SStrgUpdater_Trivial => SStrgUpdater trivial_sstorage_updater trivial_sstorage_updater_snd
+    | SStrgUpdater_Basic => SStrgUpdater basic_sstorage_updater basic_sstorage_updater_snd
+  end.
+
+
+
+  
+  (* Memory comparators *)
+  Inductive smemory_cmp_v :=
+  | SMemCmp (f: smemory_cmp_ext_t) (H_snd: safe_smemory_cmp_ext_wrt_sstack_value_cmp f).
+
+  Inductive available_memory_cmp :=
+  | SMemCmp_Trivial
+  | SMemCmp_Basic.
+
+  Definition get_memory_cmp (tag: available_memory_cmp) : smemory_cmp_v :=
+    match tag with
+    | SMemCmp_Trivial => SMemCmp trivial_memory_cmp trivial_memory_cmp_snd
+    | SMemCmp_Basic => SMemCmp basic_memory_cmp basic_memory_cmp_snd
+  end.
+
+  (* Storage comparators *)
+  Inductive sstorage_cmp_v :=
+  | SStrgCmp (f: sstorage_cmp_ext_t) (H_snd: safe_sstorage_cmp_ext_wrt_sstack_value_cmp f).
+
+  Inductive available_storage_cmp :=
+  | SStrgCmp_Trivial
+  | SStrgCmp_Basic.
+
+  Definition get_storage_cmp (tag: available_storage_cmp) : sstorage_cmp_v :=
+    match tag with
+    | SStrgCmp_Trivial => SStrgCmp trivial_storage_cmp trivial_storage_cmp_snd
+    | SStrgCmp_Basic => SStrgCmp basic_storage_cmp basic_storage_cmp_snd
+  end.
+
+
+  (* SHA3 comparators *)
+  Inductive sha3_cmp_v :=
+  | SHA3Cmp (f: sha3_cmp_ext_t) (H_snd: safe_sha3_cmp_ext_wrt_sstack_value_cmp f).
+
+  Inductive available_sha3_cmp :=
+  | SHA3Cmp_Trivial.
+
+  Definition get_sha3_cmp (tag: available_sha3_cmp) : sha3_cmp_v :=
+    match tag with
+    | SHA3Cmp_Trivial => SHA3Cmp  trivial_sha3_cmp trivial_sha3_cmp_snd
+  end.
+
+
+  (* sstack_val comparators *)
+  Inductive sstack_val_cmp_v :=
+  | SStackValCmp (f: sstack_val_cmp_ext_2_t) (H_snd: safe_sstack_value_cmp_wrt_others f) (H_d0_snd: sstack_val_cmp_fail_for_d_eq_0 f).
+
+  Inductive available_sstack_val_cmp :=
+  | SStackValCmp_Trivial
+  | SStackValCmp_Basic.
+
+  Definition get_sstack_val_cmp (tag: available_sstack_val_cmp) : sstack_val_cmp_v :=
+    match tag with
+    | SStackValCmp_Trivial => SStackValCmp trivial_compare_sstack_val trivial_compare_sstack_val_snd trivial_compare_sstack_val_d0_snd
+    | SStackValCmp_Basic => SStackValCmp basic_compare_sstack_val basic_compare_sstack_val_snd basic_compare_sstack_val_d0_snd
+  end.
+
+
+
+Definition evm_eq_block_chkr
+  (smem_updater: smemory_updater_ext_type) 
+  (sstrg_updater: sstorage_updater_ext_type)
+  (mload_solver: mload_solver_ext_type) 
+  (sload_solver: sload_solver_ext_type)
+  (sstack_value_cmp_ext: sstack_val_cmp_ext_2_t)
+  (smemory_cmp_ext: smemory_cmp_ext_t)
+  (sstorage_cmp_ext: sstorage_cmp_ext_t)
+  (sha3_cmp_ext: sha3_cmp_ext_t)
+  (opt: optim)
+  (opt_p p: block)
+  (k: nat) 
+  : bool :=
+  let sstack_value_cmp_1 := sstack_value_cmp_ext smemory_cmp_ext sstorage_cmp_ext sha3_cmp_ext in
+  let smem_updater' := smem_updater sstack_value_cmp_1 in
+  let sstrg_updater' := sstrg_updater sstack_value_cmp_1 in
+  let mload_solver' := mload_solver sstack_value_cmp_1 in
+  let sload_solver' := sload_solver sstack_value_cmp_1 in
+  match evm_sym_exec smem_updater' sstrg_updater' mload_solver' sload_solver' opt_p k evm_stack_opm with
+  | None => false
+  | Some sst_opt => 
+      match evm_sym_exec smem_updater' sstrg_updater' mload_solver' sload_solver' p k evm_stack_opm with 
+      | None => false
+      | Some sst_p => let (sst_opt', _) := opt sst_opt in 
+                      let (sst_p',   _) := opt sst_p in
+                      let d := S (max (get_maxidx_smap (get_smap_sst sst_opt')) (get_maxidx_smap (get_smap_sst sst_p'))) in
+                      let sstack_value_cmp := sstack_value_cmp_1 d in
+                      let smemory_cmp := smemory_cmp_ext sstack_value_cmp in
+                      let sstorage_cmp := sstorage_cmp_ext sstack_value_cmp in
+                      sstate_cmp sstack_value_cmp smemory_cmp sstorage_cmp sst_p' sst_opt' evm_stack_opm
+      end
+  end.
+
+
+
+End BlockEquivChecker.
